go.mod
@@ -1,6 +1,6 @@
 module github.com/nikhilc1527/HashTrieMap-Proof
 
-go 1.25.5
+go 1.26
 
 tool (
 	github.com/goose-lang/goose/cmd/goose
@@ -12,20 +12,20 @@ require (
 	github.com/bahlo/generic-list-go v0.2.0 // indirect
 	github.com/buger/jsonparser v1.1.1 // indirect
 	github.com/fatih/color v1.18.0 // indirect
-	github.com/goose-lang/goose v0.10.0 // indirect
-	github.com/goose-lang/goose/testdata/examples v0.0.0-20260114144019-e2b3e17e95c7 // indirect
+	github.com/goose-lang/goose v0.10.1-0.20260305200403-306f36d719c6 // indirect
+	github.com/goose-lang/goose/testdata/examples v0.0.0-20260224162648-279bc2d6db51 // indirect
 	github.com/inconshreveable/mousetrap v1.1.0 // indirect
 	github.com/mattn/go-colorable v0.1.14 // indirect
 	github.com/mattn/go-isatty v0.0.20 // indirect
-	github.com/mit-pdos/perennial-cli v0.4.2 // indirect
+	github.com/mit-pdos/perennial-cli v0.4.3 // indirect
 	github.com/pb33f/ordered-map/v2 v2.3.0 // indirect
 	github.com/pelletier/go-toml/v2 v2.2.4 // indirect
 	github.com/pkg/errors v0.9.1 // indirect
 	github.com/spf13/cobra v1.10.2 // indirect
 	github.com/spf13/pflag v1.0.10 // indirect
 	go.yaml.in/yaml/v4 v4.0.0-rc.3 // indirect
-	golang.org/x/mod v0.24.0 // indirect
-	golang.org/x/sync v0.13.0 // indirect
-	golang.org/x/sys v0.32.0 // indirect
-	golang.org/x/tools v0.32.0 // indirect
+	golang.org/x/mod v0.33.0 // indirect
+	golang.org/x/sync v0.19.0 // indirect
+	golang.org/x/sys v0.41.0 // indirect
+	golang.org/x/tools v0.42.0 // indirect
 )
